PREFIX acl: <http://www.w3.org/ns/auth/acl#>
PREFIX acp: <http://www.w3.org/ns/solid/acp#>
PREFIX bibo: <http://purl.org/ontology/bibo/>
PREFIX as: <https://www.w3.org/ns/activitystreams#>
PREFIX dcterms: <http://purl.org/dc/terms/>
PREFIX dpv: <https://w3id.org/dpv#>
PREFIX dpv-tech: <https://w3id.org/dpv/dpv-tech#>
PREFIX foaf: <http://xmlns.com/foaf/0.1/>
PREFIX oac: <https://w3id.org/oac#>
PREFIX odrl: <http://www.w3.org/ns/odrl/2/>
PREFIX owl: <http://www.w3.org/2002/07/owl#>
PREFIX rdf: <http://www.w3.org/1999/02/22-rdf-syntax-ns#>
PREFIX rdfs: <http://www.w3.org/2000/01/rdf-schema#>
PREFIX skos: <http://www.w3.org/2004/02/skos/core#>
PREFIX sw: <http://www.w3.org/2003/06/sw-vocab-status/ns#>
PREFIX vann: <http://purl.org/vocab/vann/>
PREFIX xsd: <http://www.w3.org/2001/XMLSchema#>

PREFIX plasma: <https://w3id.org/plasma#>

# ------------ Ontology Metadata ------------------ #

<https://w3id.org/plasma> a owl:Ontology ;
	dcterms:title "Policy Language for Solid's Metadata-based Access Control"@en ;
	vann:preferredNamespacePrefix "plasma" ;
    vann:preferredNamespaceUri "https://w3id.org/plasma#" ;
	rdfs:label "Policy Language for Solid's Metadata-based Access Control"@en ;
	owl:versionInfo "0.1"^^xsd:decimal ;
    owl:versionIRI <https://w3id.org/plasma/0.1> ;
	dcterms:created "2022-11-01"^^xsd:date ;
    dcterms:modified "2023-09-29"^^xsd:date ;
    dcterms:issued "2023-09-29"^^xsd:date ;
	dcterms:creator "Beatriz Esteves", "Harshvardhan J. Pandit" ;
    dcterms:publisher "Beatriz Esteves" ;
    dcterms:abstract "Currently, the Solid protocol and its specifications lack the terms to express metadata related to the entities, roles, processes or infrastructure necessary to provide transparency to its data handling practices. In particular, these specifications do not have the terms to deal with the obligations and requirements brought by regulations related to (personal) data protection and privacy. The establishment of a metadata language such as PLASMA enables this by providing consistent taxonomies to describe the entities (e.g., providers, developers), the infrastructure, legal roles, policies, notices, registries and logs necessary to understand and establish responsibilities and accountability within the Solid ecosystem."@en ;
	dcterms:description "Currently, the Solid protocol and its specifications lack the terms to express metadata related to the entities, roles, processes or infrastructure necessary to provide transparency to its data handling practices. In particular, these specifications do not have the terms to deal with the obligations and requirements brought by regulations related to (personal) data protection and privacy. The establishment of a metadata language such as PLASMA enables this by providing consistent taxonomies to describe the entities (e.g., providers, developers), the infrastructure, legal roles, policies, notices, registries and logs necessary to understand and establish responsibilities and accountability within the Solid ecosystem."@en ;
	rdfs:comment "This is the Turtle serialisation for PLASMA."@en ;
    dcterms:bibliographicCitation "Cite this vocabulary as: Esteves, B., & Pandit, H. J. (2023). Policy Language for Solid's Metadata-based Access Control 0.1. https://doi.org/10.5281/zenodo.10259727"@en ;
    bibo:doi "10.5281/zenodo.10259727"@en ;
	foaf:logo <https://harshp.com/plasma/img/base.png> ;
	sw:status "stable"@en ;
    dcterms:source <https://w3id.org/oac>, <https://w3id.org/dpv>, <http://www.w3.org/ns/solid/acp#> ;
    dcterms:license <https://dalicc.net/licenselibrary/CC-BY-4.0> .

# ------------ Base Concepts ------------------ #

plasma:App a rdfs:Class ;
    rdfs:isDefinedBy plasma: ;
    rdfs:label "Application"@en ;
    rdfs:subClassOf dpv-tech:Application ;
    skos:definition "An application that stores, collects, uses, shares, erases, or performs other actions on Data with the aim of providing specific purposes, services, or functionalities. An application can use several Services and requires human intervention."@en ;
    rdfs:comment "An application that stores, collects, uses, shares, erases, or performs other actions on Data with the aim of providing specific purposes, services, or functionalities. An application can use several Services and requires human intervention."@en ;
    skos:example "A Contact Address Book application or a Chess Game application"@en .

plasma:Service a rdfs:Class ;
    rdfs:isDefinedBy plasma: ;
    rdfs:label "Service"@en ;
    rdfs:subClassOf dpv-tech:Service ;
    skos:definition "A functionality that may or may not utilise or interact with Data within a Pod. Services represent an abstraction of functionality that does not necessarily have to be packaged as an App."@en ;
    rdfs:comment "A functionality that may or may not utilise or interact with Data within a Pod. Services represent an abstraction of functionality that does not necessarily have to be packaged as an App."@en ;
    skos:note "We envision service as being something that does not require the full metadata and agent-based identification and authorisation as an App. The exact mechanism for this as well as workflows for how it should be initiated and used have not been explored yet. We specify this concept to denote the possibility of having services separate from apps."@en ;
    skos:example "An Identity Verification service that checks the validity of certificates, or a Query service that retrieves contacts matching the filter"@en .

plasma:Pod a rdfs:Class ;
    rdfs:isDefinedBy plasma: ;
    rdfs:label "Pod"@en ;
    skos:altLabel "Personal Data Store"@en ;
    skos:definition "A Personal Data Store or a 'Pod' that conforms to the Solid specifications."@en ;
    rdfs:comment "A Personal Data Store or a 'Pod' that conforms to the Solid specifications."@en .

plasma:Agent a rdfs:Class ;
    rdfs:isDefinedBy plasma: ;
    rdfs:label "Agent"@en ;
    rdfs:subClassOf foaf:Agent ;
    skos:definition "A virtual entity associated with carrying out actions within or related to a Pod or its Data."@en ;
    rdfs:comment "A virtual entity associated with carrying out actions within or related to a Pod or its Data."@en .

plasma:Policy a rdfs:Class ;
    rdfs:isDefinedBy plasma: ;
    rdfs:label "Policy"@en ;
    rdfs:subClassOf odrl:Policy ;
    skos:related acp:Policy ;
    skos:definition "A set of guidelines or decisions or recommendations governing the use of Pod or its Data."@en ;
    rdfs:comment "A set of guidelines or decisions or recommendations governing the use of Pod or its Data."@en .

plasma:Data a rdfs:Class ;
    rdfs:isDefinedBy plasma: ;
    rdfs:label "Data"@en ;
    rdfs:subClassOf dpv:Data ;
    skos:definition "Data stored on a Pod or associated with User, App, Service, or Data Subject of a Pod."@en ;
    rdfs:comment "Data stored on a Pod or associated with User, App, Service, or Data Subject of a Pod."@en .

plasma:Entity a rdfs:Class ;
    rdfs:isDefinedBy plasma: ;
    rdfs:label "Entity"@en ;
    rdfs:subClassOf dpv:Entity ;
    skos:definition "A legally recognised entity. Legally recognised means the entity has some recognition as being able to enter into agreements, has an address for accountability, is responsible for obligations, rights, etc. Entities are associated with Apps, Services or Pods."@en ;
    rdfs:comment "A legally recognised entity. Legally recognised means the entity has some recognition as being able to enter into agreements, has an address for accountability, is responsible for obligations, rights, etc. Entities are associated with Apps, Services or Pods."@en .

plasma:Provider a rdfs:Class ;
    rdfs:subClassOf plasma:Entity ;
    rdfs:isDefinedBy plasma: ;
    rdfs:label "Provider"@en ;
    skos:definition "An Entity that provides some thing such as a Pod, SolidPlatform, App, Service, or Data."@en ;
    rdfs:comment "An Entity that provides some thing such as a Pod, SolidPlatform, App, Service, or Data."@en .

plasma:Developer a rdfs:Class ;
    rdfs:subClassOf plasma:Entity ;
    rdfs:isDefinedBy plasma: ;
    rdfs:label "Developer"@en ;
    skos:definition "An Entity that develops some thing such as a Pod, SolidPlatform, App, or Service."@en ;
    rdfs:comment "An Entity that develops some thing such as a Pod, SolidPlatform, App, or Service."@en .

plasma:Customer a rdfs:Class ;
    rdfs:subClassOf plasma:Entity ;
    rdfs:isDefinedBy plasma: ;
    rdfs:label "Customer"@en ;
    skos:definition "An Entity that has a business relationship with others entities to use Pods or related resources, with or without monetary transactions."@en ;
    rdfs:comment "An Entity that has a business relationship with others entities to use Pods or related resources, with or without monetary transactions."@en ;
    skos:example "Entities who purchase, lease, subscribe, or establish any form of contract or agreement for the use of Solid Pods or its related resources."@en .

plasma:SolidPlatform a rdfs:Class ;
    rdfs:isDefinedBy plasma: ;
    rdfs:label "Solid Platform"@en ;
    skos:definition "The specific implementation of Solid that is installed or used within a Pod."@en ;
    rdfs:comment "The specific implementation of Solid that is installed or used within a Pod."@en .

plasma:SolidSpecification a rdfs:Class ;
    rdfs:isDefinedBy plasma: ;
    rdfs:label "Solid Specification"@en ;
    skos:definition "The specification that the Pod conforms to in terms of defining the terms, behaviour, and implementation details regarding Pods and their association with Services and Apps."@en ;
    rdfs:comment "The specification that the Pod conforms to in terms of defining the terms, behaviour, and implementation details regarding Pods and their association with Services and Apps."@en .

# ------------ Policy Concepts ------------------ #

plasma:DataRequest a rdfs:Class ;
    rdfs:subClassOf plasma:Policy ;
    rdfs:isDefinedBy plasma: ;
    rdfs:label "Data Request"@en ;
    skos:related odrl:Request ;
    skos:definition "Request from an App, Service, Agent or User to store, collect, use, share, erase, or perform other actions on Data."@en ;
    rdfs:comment "Request from an App, Service, Agent or User to store, collect, use, share, erase, or perform other actions on Data."@en .

plasma:AppManifest a rdfs:Class ;
    rdfs:subClassOf plasma:Policy ;
    rdfs:isDefinedBy plasma: ;
    rdfs:label "App Manifest"@en ;
    skos:definition "Manifest from an App including information regarding startup parameters, identity, privacy policies and DataRequests."@en ;
    rdfs:comment "Manifest from an App including information regarding startup parameters, identity, privacy policies and DataRequests."@en .

plasma:ServiceManifest a rdfs:Class ;
    rdfs:subClassOf plasma:Policy ;
    rdfs:isDefinedBy plasma: ;
    rdfs:label "Service Manifest"@en ;
    skos:definition "Manifest from an Service including metadata, Apps using the service and information regarding DataRequests."@en ;
    rdfs:comment "Manifest from an Service including metadata, Apps using the service and information regarding DataRequests."@en .

plasma:UserPreference a rdfs:Class ;
    rdfs:subClassOf plasma:Policy ;
    rdfs:isDefinedBy plasma: ;
    rdfs:label "User Preference"@en ;
    skos:related oac:PreferencePolicy ;
    skos:definition "Preference of a User regarding purposes, entities, and other actions on Data. A preference is a soft rule that may not be satisfied."@en ;
    rdfs:comment "Preference of a User regarding purposes, entities, and other actions on Data. A preference is a soft rule that may not be satisfied."@en ;
    skos:example "When the user's preferences do not match the app's, the user can still decide to accept the stated purposes."@en .

plasma:UserRequirement a rdfs:Class ;
    rdfs:subClassOf plasma:Policy ;
    rdfs:isDefinedBy plasma: ;
    rdfs:label "User Requirement"@en ;
    skos:related oac:RequirementPolicy ;
    skos:definition "Requirements of a User regarding purposes, entities, and other actions on Data. A requirement is a hard rule that should always be satisfied."@en ;
    rdfs:comment "Requirements of a User regarding purposes, entities, and other actions on Data. A requirement is a hard rule that should always be satisfied."@en ;
    skos:example "The user requirement is to never share something - then even if the user accepts the stated request, this should not be allowed."@en .

plasma:UserOffer a rdfs:Class ;
    rdfs:subClassOf plasma:Policy ;
    rdfs:isDefinedBy plasma: ;
    rdfs:label "User Offer"@en ;
    skos:related odrl:Offer ;
    skos:definition "An offer from the User of a Pod regarding purposes, entities, and actions on Data."@en ;
    rdfs:comment "An offer from the User of a Pod regarding purposes, entities, and actions on Data."@en ;
    skos:example "The User expresses an UserOffer that their ServiceUsageStatistics as a category of Data is available for Research as a Purpose but only by NonProfitEntity (e.g. Universities), and with the requirement that it follows a specific Law (e.g. GDPR)."@en .

plasma:DataAgreement a rdfs:Class ;
    rdfs:subClassOf plasma:Policy ;
    rdfs:isDefinedBy plasma: ;
    rdfs:label "Data Agreement"@en ;
    skos:related odrl:Agreement ;
    skos:definition "An agreement regarding purposes, entities, and actions on Data."@en ;
    rdfs:comment "An agreement regarding purposes, entities, and actions on Data."@en ;
    skos:example "Stating that the User has given Consent to an App to Collect, Store, and Use some Data for a Purpose. Or, stating that the User has accepted that their Data will be Collected and Used for a providing a Service."@en .

# ------------ Agreement Concepts ------------------ #

plasma:UserConsent a rdfs:Class ;
    rdfs:subClassOf plasma:DataAgreement ;
    rdfs:isDefinedBy plasma: ;
    rdfs:label "User Consent"@en ;
    skos:definition "Agreement between a User and an Entity regarding the processing of Data in a Pod and based on the User's consent."@en ;
    rdfs:comment "Agreement between a User and an Entity regarding the processing of Data in a Pod and based on the User's consent."@en .

plasma:AppAgreement a rdfs:Class ;
    rdfs:subClassOf plasma:DataAgreement ;
    rdfs:isDefinedBy plasma: ;
    rdfs:label "App Agreement"@en ;
    skos:definition "Agreement between a User and an Entity regarding the processing of Data in a Pod and based on a contract between the User and the Entity having responsibility for the App."@en ;
    rdfs:comment "Agreement between a User and an Entity regarding the processing of Data in a Pod and based on a contract between the User and the Entity having responsibility for the App."@en .

plasma:ServiceAgreement a rdfs:Class ;
    rdfs:subClassOf plasma:DataAgreement ;
    rdfs:isDefinedBy plasma: ;
    rdfs:label "Service Agreement"@en ;
    skos:definition "Agreement between a User and an Entity regarding the processing of Data in a Pod and based on a contract between the User and the Entity having responsibility for the Service."@en ;
    rdfs:comment "Agreement between a User and an Entity regarding the processing of Data in a Pod and based on a contract between the User and the Entity having responsibility for the Service."@en .

plasma:PodAgreement a rdfs:Class ;
    rdfs:subClassOf plasma:DataAgreement ;
    rdfs:isDefinedBy plasma: ;
    rdfs:label "Pod Agreement"@en ;
    skos:definition "Agreement between a User and an Entity regarding the processing of Data in a Pod and based on a contract between the User and the Entity having responsibility for the Pod."@en ;
    rdfs:comment "Agreement between a User and an Entity regarding the processing of Data in a Pod and based on a contract between the User and the Entity having responsibility for the Pod."@en .

# ------------ Entity Concepts ------------------ #

plasma:InfrastructureProvider a rdfs:Class ;
    rdfs:subClassOf plasma:Provider ;
    rdfs:isDefinedBy plasma: ;
    rdfs:label "Infrastructure Provider"@en ;
    skos:definition "The Provider of infrastructure - such as storage, computing, network, domain names. The term infrastructure has a very specific and restricted meaning and should not be confused with other terms such as Services (e.g. analytics, querying) or Apps (e.g. data use dashboards)."@en ;
    rdfs:comment "The Provider of infrastructure - such as storage, computing, network, domain names. The term infrastructure has a very specific and restricted meaning and should not be confused with other terms such as Services (e.g. analytics, querying) or Apps (e.g. data use dashboards)."@en .

plasma:PodProvider a rdfs:Class ;
    rdfs:subClassOf plasma:Provider ;
    rdfs:isDefinedBy plasma: ;
    rdfs:label "Pod Provider"@en ;
    skos:definition "The Provider of a Pod. Here the term provider refers to an entity that provisions the Pod i.e. creates the necessary infrastructure, platform, and software so that the Pod can be used by the User."@en ;
    rdfs:comment "The Provider of a Pod. Here the term provider refers to an entity that provisions the Pod i.e. creates the necessary infrastructure, platform, and software so that the Pod can be used by the User."@en .

plasma:PodDeveloper a rdfs:Class ;
    rdfs:subClassOf plasma:Developer ;
    rdfs:isDefinedBy plasma: ;
    rdfs:label "Pod Developer"@en ;
    skos:definition "The Developer of a Pod. The developer may not be the provider, in which case this term will differ from PodProvider."@en ;
    rdfs:comment "The Developer of a Pod. The developer may not be the provider, in which case this term will differ from PodProvider."@en .

plasma:SolidPlatformProvider a rdfs:Class ;
    rdfs:subClassOf plasma:Provider ;
    rdfs:isDefinedBy plasma: ;
    rdfs:label "Solid Platform Provider"@en ;
    skos:definition "The Provider of a SolidPlatform. Here the term provider refers to an entity that provisions the SolidPlatform, i.e. creates the necessary infrastructure, platform, and software so that the SolidPlatform can be used by the User."@en ;
    rdfs:comment "The Provider of a SolidPlatform. Here the term provider refers to an entity that provisions the SolidPlatform, i.e. creates the necessary infrastructure, platform, and software so that the SolidPlatform can be used by the User."@en .

plasma:SolidPlatformDeveloper a rdfs:Class ;
    rdfs:subClassOf plasma:Developer ;
    rdfs:isDefinedBy plasma: ;
    rdfs:label "Solid Platform Developer"@en ;
    skos:definition "The Developer of a SolidPlatform. The developer may not be the provider, in which case this term will differ from SolidPlatformProvider."@en ;
    rdfs:comment "The Developer of a SolidPlatform. The developer may not be the provider, in which case this term will differ from SolidPlatformProvider."@en .

plasma:AppDeveloper a rdfs:Class ;
    rdfs:subClassOf plasma:Developer ;
    rdfs:isDefinedBy plasma: ;
    rdfs:label "App Developer"@en ;
    skos:definition "The developer of an App. Developer here refers to the Entity that developed the app, rather than individual members or units within the entity."@en ;
    rdfs:comment "The developer of an App. Developer here refers to the Entity that developed the app, rather than individual members or units within the entity."@en ;
    skos:example "Firefox has Mozilla as app developer."@en .

plasma:AppProvider a rdfs:Class ;
    rdfs:subClassOf plasma:Provider ;
    rdfs:isDefinedBy plasma: ;
    rdfs:label "App Provider"@en ;
    skos:definition "The Provider of an App. Here the term provider refers to the entity that enables that App to be accessed and used. The provider may not be the developer, in which case this term will differ from AppDeveloper. Examples include directly using an App from the developer's website (developer is same as provider), or using an App through an App Store or a common marketplace (developer is different from provider)."@en ;
    rdfs:comment "The Provider of an App. Here the term provider refers to the entity that enables that App to be accessed and used. The provider may not be the developer, in which case this term will differ from AppDeveloper. Examples include directly using an App from the developer's website (developer is same as provider), or using an App through an App Store or a common marketplace (developer is different from provider)."@en ;
    skos:example "Firefox has several providers as it can be directly downloaded from its website, or via package management, or come pre-installed on a system."@en .

plasma:ServiceDeveloper a rdfs:Class ;
    rdfs:subClassOf plasma:Developer ;
    rdfs:isDefinedBy plasma: ;
    rdfs:label "Service Developer"@en ;
    skos:definition "The Developer of a Service. Developer here refers to the entity that developed the Service, rather than individual members or units within the entity."@en ;
    rdfs:comment "The Developer of a Service. Developer here refers to the entity that developed the Service, rather than individual members or units within the entity."@en .

plasma:ServiceProvider a rdfs:Class ;
    rdfs:subClassOf plasma:Provider ;
    rdfs:isDefinedBy plasma: ;
    rdfs:label "Service Provider"@en ;
    skos:definition "The Provider of a Service. Here the term provider refers to the entity that enables that Service to be accessed and used. The provider may not be the developer, in which case this term will differ from ServiceDeveloper. Examples include directly using a Service from the developer's website (developer is same as provider), or using a Service through a Service Store or a common marketplace (developer is different from provider)."@en ;
    rdfs:comment "The Provider of a Service. Here the term provider refers to the entity that enables that Service to be accessed and used. The provider may not be the developer, in which case this term will differ from ServiceDeveloper. Examples include directly using a Service from the developer's website (developer is same as provider), or using a Service through a Service Store or a common marketplace (developer is different from provider)."@en .

plasma:IdentityProvider a rdfs:Class ;
    rdfs:subClassOf plasma:Provider ;
    rdfs:isDefinedBy plasma: ;
    rdfs:label "Identity Provider"@en ;
    skos:definition "The Provider of an identity service or credential. Here provider means the entity that provisions the identity mechanism. For example, the PodProvider also provides an identity credential for use with the Pod."@en ;
    rdfs:comment "The Provider of an identity service or credential. Here provider means the entity that provisions the identity mechanism. For example, the PodProvider also provides an identity credential for use with the Pod."@en .

plasma:IdentityDeveloper a rdfs:Class ;
    rdfs:subClassOf plasma:Developer ;
    rdfs:isDefinedBy plasma: ;
    rdfs:label "Identity Developer"@en ;
    skos:definition "The Developer of an identity service or credential. The developer may be different from a provider, in which case this term will differ from IdentityProvider. For example, a PodProvider uses an existing certificate creation service to provide certificates, in which case the developer would be the entity that created the certificate, while the PodProvider would be the provider for the identity."@en ;
    rdfs:comment "The Developer of an identity service or credential. The developer may be different from a provider, in which case this term will differ from IdentityProvider. For example, a PodProvider uses an existing certificate creation service to provide certificates, in which case the developer would be the entity that created the certificate, while the PodProvider would be the provider for the identity."@en .

plasma:User a rdfs:Class ;
    rdfs:subClassOf plasma:Entity ;
    rdfs:isDefinedBy plasma: ;
    rdfs:label "User"@en ;
    skos:definition "User of a Pod that can read, write, edit, erase data on a Pod. There may be multiple Users for a single Pod. Users can have limited permissions or abilities to interact with Data."@en ;
    rdfs:comment "User of a Pod that can read, write, edit, erase data on a Pod. There may be multiple Users for a single Pod. Users can have limited permissions or abilities to interact with Data."@en .

plasma:ReadUser a rdfs:Class ;
    rdfs:subClassOf plasma:User ;
    rdfs:isDefinedBy plasma: ;
    rdfs:label "Read User"@en ;
    skos:definition "User that can only read or view data."@en ;
    rdfs:comment "User that can only read or view data."@en .

plasma:WriteUser a rdfs:Class ;
    rdfs:subClassOf plasma:User ;
    rdfs:isDefinedBy plasma: ;
    rdfs:label "Write User"@en ;
    skos:definition "User that can only write or edit existing data."@en ;
    rdfs:comment "User that can only write or edit existing data."@en .

plasma:DataSubject a rdfs:Class ;
    rdfs:subClassOf dpv:DataSubject ;
    rdfs:isDefinedBy plasma: ;
    rdfs:label "Data Subject"@en ;
    skos:definition "The subject of Data within a Pod. The User may not always be the DataSubject. There may be multiple Subjects for a single Pod."@en ;
    rdfs:comment "The subject of Data within a Pod. The User may not always be the DataSubject. There may be multiple Subjects for a single Pod."@en .

plasma:PodAdmin a rdfs:Class ;
    rdfs:subClassOf plasma:User ;
    rdfs:isDefinedBy plasma: ;
    rdfs:label "Pod Admin"@en ;
    skos:definition "User of a Pod that has administrative capability to make decisions about the Pod (separate from Data in a Pod), such as deleting the Pod, changing identity or other resource providers, or other controls and decisions related to the use and maintainence of Pods."@en ;
    rdfs:comment "User of a Pod that has administrative capability to make decisions about the Pod (separate from Data in a Pod), such as deleting the Pod, changing identity or other resource providers, or other controls and decisions related to the use and maintainence of Pods."@en .

plasma:AdminUser a rdfs:Class ;
    rdfs:subClassOf plasma:User ;
    rdfs:isDefinedBy plasma: ;
    rdfs:label "Admin User"@en ;
    skos:definition "User of a Pod that has administrative capability to make decisions about Data on a Pod. The administration can scoped, such as being limited to specific data paths/categories, or can be global, i.e. applicable to all Data in the Pod."@en ;
    rdfs:comment "User of a Pod that has administrative capability to make decisions about Data on a Pod. The administration can scoped, such as being limited to specific data paths/categories, or can be global, i.e. applicable to all Data in the Pod."@en .

plasma:UserAgent a rdfs:Class ;
    rdfs:subClassOf plasma:Agent ;
    rdfs:isDefinedBy plasma: ;
    rdfs:label "User Agent"@en ;
    skos:definition "An Agent acting on behalf of the User."@en ;
    rdfs:comment "An Agent acting on behalf of the User."@en ;
    skos:example "A Service running or managed by the Pod that assists the User by matching the DataRequest with UserPreferences and UserRequirements."@en .

plasma:AppAgent a rdfs:Class ;
    rdfs:subClassOf plasma:Agent ;
    rdfs:isDefinedBy plasma: ;
    rdfs:label "App Agent"@en ;
    skos:definition "An Agent acting on behalf of an App."@en ;
    rdfs:comment "An Agent acting on behalf of an App."@en ;
    skos:example "An Agent that organizes an inbox application by email priority. "@en .

plasma:ServiceAgent a rdfs:Class ;
    rdfs:subClassOf plasma:Agent ;
    rdfs:isDefinedBy plasma: ;
    rdfs:label "Service Agent"@en ;
    skos:definition "An Agent acting on behalf of a Service."@en ;
    rdfs:comment "An Agent acting on behalf of a Service."@en ;
    skos:example "An Agent that syncs data stored in a Pod with another Pod."@en .

# ------------ Notice Concepts ------------------ #

plasma:Notice a rdfs:Class ;
    rdfs:subClassOf dpv:Notice ;
    rdfs:isDefinedBy plasma: ;
    rdfs:label "Notice"@en ;
    skos:definition "An artefact providing information about something."@en ;
    rdfs:comment "An artefact providing information about something."@en .

plasma:ExAnteNotice a rdfs:Class ;
    rdfs:subClassOf plasma:Notice ;
    rdfs:isDefinedBy plasma: ;
    rdfs:label "Ex-Ante Notice"@en ;
    skos:definition "A Notice that is provided before something happens."@en ;
    rdfs:comment "A Notice that is provided before something happens."@en .

plasma:ExPostNotice a rdfs:Class ;
    rdfs:subClassOf plasma:Notice ;
    rdfs:isDefinedBy plasma: ;
    rdfs:label "Ex-Post Notice"@en ;
    skos:definition "A Notice that is provided after something happens."@en ;
    rdfs:comment "A Notice that is provided after something happens."@en .

plasma:NoticeProvider a rdfs:Class ;
    rdfs:subClassOf plasma:Provider ;
    rdfs:isDefinedBy plasma: ;
    rdfs:label "Notice Provider"@en ;
    skos:definition "Entity that provides the Notice."@en ;
    rdfs:comment "Entity that provides the Notice."@en .

plasma:NoticeRecipient a rdfs:Class ;
    rdfs:subClassOf plasma:Entity ;
    rdfs:isDefinedBy plasma: ;
    rdfs:label "Notice Recipient"@en ;
    skos:definition "Entity that receives the Notice."@en ;
    rdfs:comment "Entity that receives the Notice."@en .

plasma:NoticeContext a rdfs:Class ;
    rdfs:isDefinedBy plasma: ;
    rdfs:label "Notice Context"@en ;
    skos:definition "Information about a Notice, such as where/when/how/why it was provided."@en ;
    rdfs:comment "Information about a Notice, such as where/when/how/why it was provided."@en .

plasma:AppPrivacyNotice a rdfs:Class ;
    rdfs:subClassOf plasma:Notice ;
    rdfs:isDefinedBy plasma: ;
    rdfs:label "App Privacy Notice"@en ;
    skos:definition "An App's privacy Notice."@en ;
    rdfs:comment "An App's privacy Notice."@en .

plasma:ServicePrivacyNotice a rdfs:Class ;
    rdfs:subClassOf plasma:Notice ;
    rdfs:isDefinedBy plasma: ;
    rdfs:label "Service Privacy Notice"@en ;
    skos:definition "A Service's privacy Notice."@en ;
    rdfs:comment "A Service's privacy Notice."@en .

plasma:PodPrivacyNotice a rdfs:Class ;
    rdfs:subClassOf plasma:Notice ;
    rdfs:isDefinedBy plasma: ;
    rdfs:label "Pod Privacy Notice"@en ;
    skos:definition "A PodProvider's or PodDeveloper's privacy Notice."@en ;
    rdfs:comment "A PodProvider's or PodDeveloper's privacy Notice."@en .

plasma:UserPrivacyNotice a rdfs:Class ;
    rdfs:subClassOf plasma:Notice ;
    rdfs:isDefinedBy plasma: ;
    rdfs:label "User Privacy Notice"@en ;
    skos:definition "A Pod User's privacy Notice regarding their Data."@en ;
    rdfs:comment "A Pod User's privacy Notice regarding their Data."@en .

# ------------ Service Concepts ------------------ #

plasma:IdentityService a rdfs:Class ;
    rdfs:subClassOf plasma:Service ;
    rdfs:isDefinedBy plasma: ;
    rdfs:label "Identity Service"@en ;
    skos:definition "A Service providing identity credentials and identifiers."@en ;
    rdfs:comment "A Service providing identity credentials and identifiers."@en .

plasma:LoggingService a rdfs:Class ;
    rdfs:subClassOf plasma:Service ;
    rdfs:isDefinedBy plasma: ;
    rdfs:label "Logging Service"@en ;
    skos:definition "A Service providing logging mechanisms and functionalities."@en ;
    rdfs:comment "A Service providing logging mechanisms and functionalities."@en .

plasma:AccessControlService a rdfs:Class ;
    rdfs:subClassOf plasma:Service ;
    rdfs:isDefinedBy plasma: ;
    rdfs:label "Access Control Service"@en ;
    skos:definition "A Service providing access control management and associated functionalities."@en ;
    rdfs:comment "A Service providing access control management and associated functionalities."@en .

plasma:PolicyManagementService a rdfs:Class ;
    rdfs:subClassOf plasma:Service ;
    rdfs:isDefinedBy plasma: ;
    rdfs:label "Policy Management Service"@en ;
    skos:definition "A Service providing policy management and resolution functionalities."@en ;
    rdfs:comment "A Service providing policy management and resolution functionalities."@en .

plasma:IdentityManagementService a rdfs:Class ;
    rdfs:subClassOf plasma:Service ;
    rdfs:isDefinedBy plasma: ;
    rdfs:label "Identity Management Service"@en ;
    skos:definition "A Service providing identity management functionalities."@en ;
    rdfs:comment "A Service providing identity management functionalities."@en .

plasma:DataManagementService a rdfs:Class ;
    rdfs:subClassOf plasma:Service ;
    rdfs:isDefinedBy plasma: ;
    rdfs:label "Data Management Service"@en ;
    skos:definition "A Service providing data management and associated functionalities."@en ;
    rdfs:comment "A Service providing data management and associated functionalities."@en .

plasma:NetworkManagementService a rdfs:Class ;
    rdfs:subClassOf plasma:Service ;
    rdfs:isDefinedBy plasma: ;
    rdfs:label "Network Management Service"@en ;
    skos:definition "A Service providing network management and associated functionalities."@en ;
    rdfs:comment "A Service providing network management and associated functionalities."@en .

plasma:DataStorageService a rdfs:Class ;
    rdfs:subClassOf plasma:Service ;
    rdfs:isDefinedBy plasma: ;
    rdfs:label "Data Storage Service"@en ;
    skos:definition "A Service providing data storage and associated functionalities."@en ;
    rdfs:comment "A Service providing data storage and associated functionalities."@en .

plasma:ComputeService a rdfs:Class ;
    rdfs:subClassOf plasma:Service ;
    rdfs:isDefinedBy plasma: ;
    rdfs:label "Compute Service"@en ;
    skos:definition "A Service providing computing and associated functionalities."@en ;
    rdfs:comment "A Service providing computing and associated functionalities."@en .

plasma:DataQueryService a rdfs:Class ;
    rdfs:subClassOf plasma:Service ;
    rdfs:isDefinedBy plasma: ;
    rdfs:label "Data Query Service"@en ;
    skos:definition "A Service providing data querying and associated functionalities."@en ;
    rdfs:comment "A Service providing data querying and associated functionalities."@en .

plasma:AppManagementService a rdfs:Class ;
    rdfs:subClassOf plasma:Service ;
    rdfs:isDefinedBy plasma: ;
    rdfs:label "App Management Service"@en ;
    skos:definition "A Service providing app management and associated functionalities."@en ;
    rdfs:comment "A Service providing app management and associated functionalities."@en .

plasma:ServiceManagement a rdfs:Class ;
    rdfs:subClassOf plasma:Service ;
    rdfs:isDefinedBy plasma: ;
    rdfs:label "Service Management"@en ;
    skos:definition "A Service providing service management and associated functionalities."@en ;
    rdfs:comment "A Service providing service management and associated functionalities."@en .

# ------------ Data Concepts ------------------ #

plasma:Log a rdfs:Class ;
    rdfs:isDefinedBy plasma: ;
    rdfs:label "Log"@en ;
    skos:definition "A provenance record associated with a process."@en ;
    rdfs:comment "A provenance record associated with a process."@en .

plasma:DataLog a rdfs:Class ;
    rdfs:subClassOf plasma:Log ;
    rdfs:isDefinedBy plasma: ;
    rdfs:label "Data Log"@en ;
    skos:definition "A Log regarding actions on Data."@en ;
    rdfs:comment "A Log regarding actions on Data."@en ;
    skos:example "When data was added / stored in the Pod, when it was erased, accessed, or queried."@en .

plasma:AccessControlLog a rdfs:Class ;
    rdfs:subClassOf plasma:Log ;
    rdfs:isDefinedBy plasma: ;
    rdfs:label "Access Control Log"@en ;
    skos:definition "A Log regarding access actions on Data."@en ;
    rdfs:comment "A Log regarding access actions on Data."@en ;
    skos:example "When data was permitted or denied to be accessed."@en .

plasma:PolicyLog a rdfs:Class ;
    rdfs:subClassOf plasma:Log ;
    rdfs:isDefinedBy plasma: ;
    rdfs:label "Policy Log"@en ;
    skos:definition "A Log regarding Policies governing the Data."@en ;
    rdfs:comment "A Log regarding Policies governing the Data."@en ;
    skos:example "A new user preference or requirement was added, or an app made a request, or a policy negotiation succefully took place and the user granted their consent."@en .

plasma:IdentityLog a rdfs:Class ;
    rdfs:subClassOf plasma:Log ;
    rdfs:isDefinedBy plasma: ;
    rdfs:label "Identity Log"@en ;
    skos:definition "A Log regarding identity provision, verification, and its use."@en ;
    rdfs:comment "A Log regarding identity provision, verification, and its use."@en ;
    skos:example "An app's identity could not be verified, or a user succeffully logged in."@en .

plasma:SecurityLog a rdfs:Class ;
    rdfs:subClassOf plasma:Log ;
    rdfs:isDefinedBy plasma: ;
    rdfs:label "Security Log"@en ;
    skos:definition "A Log regarding security concerns and incidents."@en ;
    rdfs:comment "A Log regarding security concerns and incidents."@en ;
    skos:example "Data integrity has failed a check, or there was an attempt to repeatedly access data without sufficient authorisation. "@en .

plasma:UserData a rdfs:Class ;
    rdfs:subClassOf plasma:Data ;
    rdfs:isDefinedBy plasma: ;
    rdfs:label "User Data"@en ;
    skos:definition "Data belonging or about the User."@en ;
    rdfs:comment "Data belonging or about the User."@en .

plasma:DataProvider a rdfs:Class ;
    rdfs:subClassOf plasma:Provider ;
    rdfs:isDefinedBy plasma: ;
    rdfs:label "Data Provider"@en ;
    skos:related dpv:DataSource ;
    skos:definition "The provider or source of data. It can be made available by the User or a data provider or can be generated by an App, Service or Agent."@en ;
    rdfs:comment "The provider or source of data. It can be made available by the User or a data provider or can be generated by an App, Service or Agent."@en .

plasma:ResourceMetadata a rdfs:Class ;
    rdfs:subClassOf plasma:UserData ;
    rdfs:isDefinedBy plasma: ;
    rdfs:label "Resource Metadata"@en ;
    skos:definition "Information about the Data contained in a Pod resource."@en ;
    rdfs:comment "Information about the Data contained in a Pod resource."@en ;
    skos:example "Resource A contains health data or resource B was updated by User X on date YYYY-MM-DD."@en .

plasma:AppData a rdfs:Class ;
    rdfs:subClassOf plasma:Data ;
    rdfs:isDefinedBy plasma: ;
    rdfs:label "App Data"@en ;
    skos:definition "Data required by an App to provide its functionalities, or recording relevant contextual information."@en ;
    rdfs:comment "Data required by an App to provide its functionalities, or recording relevant contextual information."@en .

plasma:AppMetadata a rdfs:Class ;
    rdfs:subClassOf plasma:AppData ;
    rdfs:isDefinedBy plasma: ;
    rdfs:label "App Metadata"@en ;
    skos:definition "Information about an App such as who was its Provider, Developer, what functionalities and services it offers, relevant policies and authorisations."@en ;
    rdfs:comment "Information about an App such as who was its Provider, Developer, what functionalities and services it offers, relevant policies and authorisations."@en .

plasma:AppLog a rdfs:Class ;
    rdfs:subClassOf plasma:AppData, plasma:Log ;
    rdfs:isDefinedBy plasma: ;
    rdfs:label "App Log"@en ;
    skos:definition "Logs related to an App's activities."@en ;
    rdfs:comment "Logs related to an App's activities."@en .

plasma:AppPersistentData a rdfs:Class ;
    rdfs:subClassOf plasma:AppData ;
    rdfs:isDefinedBy plasma: ;
    rdfs:label "App Persistent Data"@en ;
    skos:definition "Data required by the App that is persistently stored. For example, results of a frequent query."@en ;
    rdfs:comment "Data required by the App that is persistently stored. For example, results of a frequent query."@en .

plasma:AppTemporaryData a rdfs:Class ;
    rdfs:subClassOf plasma:AppData ;
    rdfs:isDefinedBy plasma: ;
    rdfs:label "App Temporary Data"@en ;
    skos:definition "Data required by the App that is temporarily stored. For example, results of a non-frequent query."@en ;
    rdfs:comment "Data required by the App that is temporarily stored. For example, results of a non-frequent query."@en .

plasma:ServiceData a rdfs:Class ;
    rdfs:subClassOf plasma:Data ;
    rdfs:isDefinedBy plasma: ;
    rdfs:label "Service Data"@en ;
    skos:definition "Data required by a Service to provide its functionalities, or recording relevant contextual information. "@en ;
    rdfs:comment "Data required by a Service to provide its functionalities, or recording relevant contextual information. "@en .

plasma:ServiceMetadata a rdfs:Class ;
    rdfs:subClassOf plasma:ServiceData ;
    rdfs:isDefinedBy plasma: ;
    rdfs:label "Service Metadata"@en ;
    skos:definition "Information about a Service such as who was its Provider, Developer, what functionalities and services it offers, relevant policies and authorisations."@en ;
    rdfs:comment "Information about a Service such as who was its Provider, Developer, what functionalities and services it offers, relevant policies and authorisations."@en .

plasma:ServiceLog a rdfs:Class ;
    rdfs:subClassOf plasma:ServiceData, plasma:Log ;
    rdfs:isDefinedBy plasma: ;
    rdfs:label "Service Log"@en ;
    skos:definition "Logs related to a Service's activities."@en ;
    rdfs:comment "Logs related to a Service's activities."@en .

plasma:ServicePersistentData a rdfs:Class ;
    rdfs:subClassOf plasma:ServiceData ;
    rdfs:isDefinedBy plasma: ;
    rdfs:label "Service Persistent Data"@en ;
    skos:definition "Data required by the Service that is persistently stored. For example, results of a frequent query."@en ;
    rdfs:comment "Data required by the Service that is persistently stored. For example, results of a frequent query."@en .

plasma:ServiceTemporaryData a rdfs:Class ;
    rdfs:subClassOf plasma:ServiceData ;
    rdfs:isDefinedBy plasma: ;
    rdfs:label "Service Temporary Data"@en ;
    skos:definition "Data required by the Service that is temporarily stored. For example, results of a non-frequent query."@en ;
    rdfs:comment "Data required by the Service that is temporarily stored. For example, results of a non-frequent query."@en .

plasma:PodManagementData a rdfs:Class ;
    rdfs:subClassOf plasma:Data ;
    rdfs:isDefinedBy plasma: ;
    rdfs:label "Pod Management Data"@en ;
    skos:definition "Data required by a Pod to provide its functionalities. For example, storing the Pod metadata regarding Provider, Developer, PodAgreement, or credentials associated with Pod infrastructure."@en ;
    rdfs:comment "Data required by a Pod to provide its functionalities. For example, storing the Pod metadata regarding Provider, Developer, PodAgreement, or credentials associated with Pod infrastructure."@en .

plasma:SchemaData a rdfs:Class ;
    rdfs:subClassOf plasma:Data ;
    rdfs:isDefinedBy plasma: ;
    rdfs:label "Schema Data"@en ;
    skos:definition "Schemas, formats or shapes for the Data recognised or supported by Apps, Services or Pods."@en ;
    rdfs:comment "Schemas, formats or shapes for the Data recognised or supported by Apps, Services or Pods."@en .

plasma:Registry a rdfs:Class ;
    rdfs:isDefinedBy plasma: ;
    rdfs:label "Registry"@en ;
    skos:definition "An indexed record for providing collective and convenient access to Data within a Pod."@en ;
    rdfs:comment "An indexed record for providing collective and convenient access to Data within a Pod."@en .

plasma:AccessControlRegistry a rdfs:Class ;
    rdfs:subClassOf plasma:Registry ;
    rdfs:isDefinedBy plasma: ;
    rdfs:label "Access Control Registry"@en ;
    skos:definition "A Registry listing access control decisions and authorisations."@en ;
    rdfs:comment "A Registry listing access control decisions and authorisations."@en .

plasma:DataRegistry a rdfs:Class ;
    rdfs:subClassOf plasma:Registry ;
    rdfs:isDefinedBy plasma: ;
    rdfs:label "Data Registry"@en ;
    skos:definition "A Registry listing data categories, resources, availability, and other relevant information."@en ;
    rdfs:comment "A Registry listing data categories, resources, availability, and other relevant information."@en .

plasma:DataSchemaRegistry a rdfs:Class ;
    rdfs:subClassOf plasma:Registry ;
    rdfs:isDefinedBy plasma: ;
    rdfs:label "Data Schema Registry"@en ;
    skos:definition "A Registry listing recognised or supported SchemaData for Pods, Apps, or Services."@en ;
    rdfs:comment "A Registry listing recognised or supported SchemaData for Pods, Apps, or Services."@en .

plasma:PolicyRegistry a rdfs:Class ;
    rdfs:subClassOf plasma:Registry ;
    rdfs:isDefinedBy plasma: ;
    rdfs:label "Policy Registry"@en ;
    skos:definition "A Registry listing policies relevant to Data, Apps, Services, and Pod. For example, user preferences, consent decisions, pending requests."@en ;
    rdfs:comment "A Registry listing policies relevant to Data, Apps, Services, and Pod. For example, user preferences, consent decisions, pending requests."@en .

plasma:AppRegistry a rdfs:Class ;
    rdfs:subClassOf plasma:Registry ;
    rdfs:isDefinedBy plasma: ;
    rdfs:label "App Registry"@en ;
    skos:definition "A Registry listing Apps associated with the Pod. For example, a contact book app along with its relevant metadata such as Provider, Developer, Policies."@en ;
    rdfs:comment "A Registry listing Apps associated with the Pod. For example, a contact book app along with its relevant metadata such as Provider, Developer, Policies."@en .

plasma:ServiceRegistry a rdfs:Class ;
    rdfs:subClassOf plasma:Registry ;
    rdfs:isDefinedBy plasma: ;
    rdfs:label "Service Registry"@en ;
    skos:definition "A Registry listing Services associated with the Pod. For example, a query service that can retrieve data along with its relevant metadata such as Provider, Developer, Policies."@en ;
    rdfs:comment "A Registry listing Services associated with the Pod. For example, a query service that can retrieve data along with its relevant metadata such as Provider, Developer, Policies."@en .

plasma:UserRegistry a rdfs:Class ;
    rdfs:subClassOf plasma:Registry ;
    rdfs:isDefinedBy plasma: ;
    rdfs:label "User Registry"@en ;
    skos:definition "A Registry listing Users associated with the Pod and their relevant Policies, Agents, and other relevant information."@en ;
    rdfs:comment "A Registry listing Users associated with the Pod and their relevant Policies, Agents, and other relevant information."@en .

# ------------ Activity types ------------------ #

plasma:Request a owl:Class ;
    rdfs:subClassOf as:Activity ;
    rdfs:isDefinedBy plasma: ;
    rdfs:label "Request"@en ;
    skos:definition "To request some data."@en ;
    rdfs:comment "To request some data."@en .

plasma:Login a owl:Class ;
    rdfs:subClassOf as:Activity ;
    rdfs:isDefinedBy plasma: ;
    rdfs:label "Login"@en ;
    skos:definition "To successfully login."@en ;
    rdfs:comment "To successfully login."@en .

plasma:Verify a owl:Class ;
    rdfs:subClassOf as:Activity ;
    rdfs:isDefinedBy plasma: ;
    rdfs:label "Verify"@en ;
    skos:definition "To verify something."@en ;
    rdfs:comment "To verify something."@en .

plasma:ChangeIdP a owl:Class ;
    rdfs:subClassOf as:Activity ;
    rdfs:isDefinedBy plasma: ;
    rdfs:label "Change identity provider"@en ;
    skos:definition "To change identity provider."@en ;
    rdfs:comment "To change identity provider."@en .

# ------------ Properties ------------------ #

plasma:hasProvider a rdf:Property ;
	rdfs:isDefinedBy plasma: ;
	rdfs:label "Has provider"@en ;
	skos:definition "Indicates association with the provider of a Pod, Solid platform or infrastructure, identity, app, service or data."@en ;
    rdfs:comment "Indicates association with the provider of a Pod, Solid platform or infrastructure, identity, app, service or data."@en ;
	rdfs:range plasma:Provider .

plasma:hasDeveloper a rdf:Property ;
	rdfs:isDefinedBy plasma: ;
	rdfs:label "Has developer"@en ;
	skos:definition "Indicates association with the developer of a Pod, Solid platform, identity, app or service."@en ;
    rdfs:comment "Indicates association with the developer of a Pod, Solid platform, identity, app or service."@en ;
    rdfs:range plasma:Developer .

plasma:implementedSolidPlatform a rdf:Property ;
	rdfs:isDefinedBy plasma: ;
	rdfs:label "Implemented using Solid platform"@en ;
	skos:definition "Indicates the Solid platform that is installed or used within a Pod."@en ;
    rdfs:comment "Indicates the Solid platform that is installed or used within a Pod."@en ;
	rdfs:domain plasma:PodManagementData ;
	rdfs:range plasma:SolidPlatform .

plasma:implementedSolidSpecification a rdf:Property ;
	rdfs:isDefinedBy plasma: ;
	rdfs:label "Implemented using Solid specification"@en ;
	skos:definition "Indicates the Solid specification that the Pod conforms to."@en ;
    rdfs:comment "Indicates the Solid specification that the Pod conforms to."@en ;
	rdfs:domain plasma:PodManagementData ;
	rdfs:range plasma:SolidSpecification .

plasma:serviceType a rdf:Property ;
	rdfs:isDefinedBy plasma: ;
	rdfs:label "Service type"@en ;
	skos:definition "Indicates the type of service provided/developed by a service provider/developer."@en ;
    rdfs:comment "Indicates the type of service provided/developed by a service provider/developer."@en ;
	rdfs:domain plasma:ServiceProvider, plasma:ServiceDeveloper ;
	rdfs:range plasma:Service .

plasma:serviceProvidedByApp a rdf:Property ;
	rdfs:isDefinedBy plasma: ;
	rdfs:label "Service provided by App"@en ;
	skos:definition "Indicates an app that uses a particular service to provide a certain functionality."@en ;
    rdfs:comment "Indicates an app that uses a particular service to provide a certain functionality."@en ;
	rdfs:domain plasma:Service ;
	rdfs:range plasma:App .

plasma:hasAuthorisation a rdf:Property ;
	rdfs:isDefinedBy plasma: ;
	rdfs:label "Has authorisation"@en ;
	skos:definition "Indicates an access control authorisation."@en ;
    rdfs:comment "Indicates an access control authorisation."@en ;
	rdfs:domain plasma:AccessControlRegistry ;
	rdfs:range acl:Authorization , acp:AccessGrant .

plasma:hasSchema a rdf:Property ;
	rdfs:isDefinedBy plasma: ;
	rdfs:label "Has schema"@en ;
	skos:definition "Indicates a schema, format or shape for data."@en ;
    rdfs:comment "Indicates a schema, format or shape for data."@en ;
	rdfs:domain plasma:DataSchemaRegistry ;
	rdfs:range plasma:SchemaData .

plasma:supportedBy a rdf:Property ;
	rdfs:isDefinedBy plasma: ;
	rdfs:label "Supported by"@en ;
	skos:definition "Indicates an app, service or Pod that supports a particular schema, format or shape for data."@en ;
    rdfs:comment "Indicates an app, service or Pod that supports a particular schema, format or shape for data."@en ;
	rdfs:domain plasma:SchemaData ;
	rdfs:range plasma:App, plasma:Service, plasma:Pod .

plasma:hasUser a rdf:Property ;
	rdfs:isDefinedBy plasma: ;
	rdfs:label "Has user"@en ;
	skos:definition "Indicates association with a user."@en ;
    rdfs:comment "Indicates association with a user."@en ;
	rdfs:domain plasma:UserRegistry ;
	rdfs:range plasma:User .

plasma:hasPolicy a rdf:Property ;
	rdfs:isDefinedBy plasma: ;
	rdfs:label "Has user"@en ;
	skos:definition "Indicates association of an entity with a policy."@en ;
    rdfs:comment "Indicates association of an entity with a policy."@en ;
	rdfs:domain plasma:Entity ;
	rdfs:range plasma:Policy .

plasma:hasAgent a rdf:Property ;
	rdfs:isDefinedBy plasma: ;
	rdfs:label "Has agent"@en ;
	skos:definition "Indicates association of an user, app or service with an agent acting on its behalf."@en ;
    rdfs:comment "Indicates association of an user, app or service with an agent acting on its behalf."@en ;
	rdfs:domain plasma:User, plasma:App, plasma:Service ;
	rdfs:range plasma:Agent .

plasma:hasAppManifest a rdf:Property ;
	rdfs:isDefinedBy plasma: ;
	rdfs:label "Has application manifest"@en ;
	skos:definition "Indicates association of an app with an app manifest."@en ;
    rdfs:comment "Indicates association of an app with an app manifest."@en ;
	rdfs:domain plasma:App ;
	rdfs:range plasma:AppManifest .

plasma:hasApp a rdf:Property ;
	rdfs:isDefinedBy plasma: ;
	rdfs:label "Has app"@en ;
	skos:definition "Indicates association with an app."@en ;
    rdfs:comment "Indicates association with an app."@en ;
	rdfs:domain plasma:AppRegistry ;
	rdfs:range plasma:App .

plasma:hasAppMetadata a rdf:Property ;
	rdfs:isDefinedBy plasma: ;
	rdfs:label "Has app metadata"@en ;
	skos:definition "Indicates association with app metadata."@en ;
    rdfs:comment "Indicates association with app metadata."@en ;
	rdfs:domain plasma:App ;
	rdfs:range plasma:AppMetadata .

plasma:hasAppPersistentData a rdf:Property ;
	rdfs:isDefinedBy plasma: ;
	rdfs:label "Has app persistent data"@en ;
	skos:definition "Indicates association with app data that is persistently stored in the Pod."@en ;
    rdfs:comment "Indicates association with app data that is persistently stored in the Pod."@en ;
	rdfs:domain plasma:App ;
	rdfs:range plasma:AppPersistentData .

plasma:hasAppTemporaryData a rdf:Property ;
	rdfs:isDefinedBy plasma: ;
	rdfs:label "Has app temporary data"@en ;
	skos:definition "Indicates association with app data that is temporarily stored in the Pod."@en ;
    rdfs:comment "Indicates association with app data that is temporarily stored in the Pod."@en ;
	rdfs:domain plasma:App ;
	rdfs:range plasma:AppTemporaryData .

plasma:hasServiceManifest a rdf:Property ;
	rdfs:isDefinedBy plasma: ;
	rdfs:label "Has service manifest"@en ;
	skos:definition "Indicates association of a service with a service manifest."@en ;
    rdfs:comment "Indicates association of a service with a service manifest."@en ;
	rdfs:domain plasma:Service ;
	rdfs:range plasma:ServiceManifest .

plasma:hasService a rdf:Property ;
	rdfs:isDefinedBy plasma: ;
	rdfs:label "Has service"@en ;
	skos:definition "Indicates association with a service."@en ;
    rdfs:comment "Indicates association with a service."@en ;
	rdfs:domain plasma:ServiceRegistry ;
	rdfs:range plasma:Service .

plasma:hasServiceMetadata a rdf:Property ;
	rdfs:isDefinedBy plasma: ;
	rdfs:label "Has service metadata"@en ;
	skos:definition "Indicates association with service metadata."@en ;
    rdfs:comment "Indicates association with service metadata."@en ;
	rdfs:domain plasma:Service ;
	rdfs:range plasma:ServiceMetadata .

plasma:hasServicePersistentData a rdf:Property ;
	rdfs:isDefinedBy plasma: ;
	rdfs:label "Has service persistent data"@en ;
	skos:definition "Indicates association with service data that is persistently stored in the Pod."@en ;
    rdfs:comment "Indicates association with service data that is persistently stored in the Pod."@en ;
	rdfs:domain plasma:Service ;
	rdfs:range plasma:ServicePersistentData .

plasma:hasServiceTemporaryData a rdf:Property ;
	rdfs:isDefinedBy plasma: ;
	rdfs:label "Has service temporary data"@en ;
	skos:definition "Indicates association with service data that is temporarily stored in the Pod."@en ;
    rdfs:comment "Indicates association with service data that is temporarily stored in the Pod."@en ;
	rdfs:domain plasma:App ;
	rdfs:range plasma:ServiceTemporaryData .